Removed vacuous spec + simplified encode/decode

src/Term.v
@@ -4,7 +4,6 @@ Unset Strict Implicit.
 Unset Printing Implicit Defensive.
 
 Import Order.Theory.
-Section Term.
 
   (* literals should be of Datatype type, is not important for the moment*)
   Open Scope order_scope.
@@ -13,7 +12,7 @@ Section Term.
   | Iri (id: I)
   | Lit (l : L)
   | Bnode (name : B).
-
+  
   Arguments Iri {I B L}.
   Arguments Lit {I B L}.
   Arguments Bnode {I B L}.
@@ -43,113 +42,170 @@ Section Term.
   Definition is_in_i (I B L : Type) (trm : term I B L) : bool :=
     is_iri trm.
 
-  Definition is_in_ibl (I B L : Type) (trm : term I B L) : bool :=
-    is_iri trm || is_bnode trm || is_lit trm.
+  (* Definition is_in_ibl (I B L : Type) (trm : term I B L) : bool := *)
+  (*   is_iri trm || is_bnode trm || is_lit trm. *)
+
+  (* (* what is the use of is_in_ibl ? *) *)
+  (* Lemma trivial_is_in_ibl I B L (t : term I B L) : is_in_ibl t. *)
+  (* Proof. by case: t => *. Qed. *)
+
+Section Poly.
+Variables I B B1 B2 B3 L : Type.
+  (* Implicit Type trm : term I B L. *)
+
+    (* Definition get_b_term trm : is_bnode trm -> B. *)
+    (* Proof. rewrite /is_bnode=> is_b. case trm eqn:E; *)
+    (*          try discriminate is_b. *)
+    (*        exact name. *)
+    (* Defined. *)
+
+Definition relabeling_term B1 B2 μ (trm : term I B1 L) : term I B2 L :=
+  match trm with
+  | Bnode name => Bnode (μ name)
+  | Iri i => Iri i
+  | Lit l => Lit l
+  end.
+
+Lemma relabeling_term_id (trm : term I B L) : relabeling_term id trm = trm.
+Proof. by case: trm. Qed.
+
+Lemma relabeling_term_comp trm (μ1: B1 -> B2) (μ2 : B2 -> B3) :
+  relabeling_term (μ2 \o μ1) trm = relabeling_term μ2 (relabeling_term μ1 trm).
+Proof. by case: trm. Qed.
+
+Lemma relabeling_term_preserves_is_in_ib (μ : B1 -> B2) (trm : term I B1 L) :
+  is_in_ib  trm <-> is_in_ib (relabeling_term μ trm).
+Proof. by case: trm. Qed.
+
+Lemma relabeling_term_preserves_is_in_i (μ : B1 -> B2) (trm : term I B1 L) :
+  is_in_i trm <-> is_in_i (relabeling_term μ trm).
+Proof. by case: trm. Qed.
+
+Lemma relabeling_term_ext (μ1 μ2 : B1 -> B2) :
+  μ1 =1 μ2 -> relabeling_term μ1 =1 relabeling_term μ2.
+Proof. by move=> μpweq [//| // | b] /=; rewrite μpweq. Qed.
+
+End Poly.
+
+Section CodeTerm.
+
+Variables (I B L : Type).
+
+Implicit Type trm : term I B L.
+
+Definition code_term trm : GenTree.tree (I + B + L)%type :=
+  match trm with
+  | Iri i => GenTree.Node 0 (GenTree.Leaf (inl (inl i)) :: nil)
+  | Lit l => GenTree.Node 1 (GenTree.Leaf (inr l) :: nil)
+  | Bnode name => GenTree.Node 2 (GenTree.Leaf (inl (inr name)) :: nil)
+  end.
+
+Definition decode_term (x : GenTree.tree (I + B + L)) : option (term I B L) :=
+  match x with
+  | GenTree.Node 0 (GenTree.Leaf (inl (inl i)) :: nil) => Some (Iri i)
+  | GenTree.Node 1 (GenTree.Leaf (inr l) :: nil) =>  Some (Lit l)
+  | GenTree.Node 2 (GenTree.Leaf (inl (inr name)) :: nil) => Some (Bnode name)
+  | _ => None
+  end.
+
+Lemma pcancel_code_decode : pcancel code_term decode_term.
+Proof. by case => [i | l | name]. Qed.
+
+End CodeTerm.
+
+Definition term_canEqMixin (I B L : eqType) := PcanEqMixin (@pcancel_code_decode I B L).
+Canonical term_eqType (I B L : eqType) :=
+  Eval hnf in EqType (term I B L) (term_canEqMixin I B L).
+
+Definition term_canChoiceMixin (I B L : choiceType) :=
+  PcanChoiceMixin (@pcancel_code_decode I B L).
+
+Canonical term_choiceType (I B L : choiceType) :=
+  Eval hnf in ChoiceType (term I B L) (term_canChoiceMixin I B L).
+
+Definition term_canCountMixin (I B L : countType) :=
+  PcanCountMixin (@pcancel_code_decode I B L).
+Canonical term_countType (I B L : countType) :=
+  Eval hnf in CountType (term I B L) (term_canCountMixin I B L).
+
+Definition term_canPOrderMixin (I B L : countType) :=
+  PcanPOrderMixin (@pickleK (term_countType I B L)).
+
+Canonical term_POrderType (I B L : countType) :=
+  Eval hnf in POrderType tt (term_countType I B L) (term_canPOrderMixin I B L).
 
 
-  Section Poly.
-    Variables I B L : Type.
-    Implicit Type trm : term I B L.
 
-    Definition get_b_term trm : is_bnode trm -> B.
-    Proof. rewrite /is_bnode=> is_b. case trm eqn:E;
-             try discriminate is_b.
-           exact name.
-    Defined.
 
-    Definition relabeling_term (B' B'' : Type) (μ : B' -> B'') (trm : (term I B' L)) : term I B'' L :=
-      match trm with
-      | Bnode name => Bnode (μ name)
-      | Iri i => Iri i
-      | Lit l => Lit l
-      end.
 
-    Lemma relabeling_term_id trm : relabeling_term id trm = trm.
-    Proof. by case trm. Qed.
+(* Definition term_canChoiceMixin := PcanChoiceMixin cancel_code_decode. *)
+(* Definition term_canCountMixin := PcanCountMixin cancel_code_decode. *)
 
-    Lemma relabeling_term_comp (B' B'' : Type) trm (μ1: B -> B') (μ2 : B' -> B'') :
-      relabeling_term (μ2 \o μ1) trm = relabeling_term μ2 (relabeling_term μ1 trm).
-    Proof. by case trm. Qed.
+(* Canonical term_choiceType := Eval hnf in ChoiceType (term I B L) term_canChoiceMixin. *)
+(* Canonical term_countType := Eval hnf in CountType (term I B L) term_canCountMixin. *)
 
-    Section Relabeling_term.
-      Variable B' : Type.
-      Implicit Type μ : B -> B'.
+(*     Definition term_canPOrderMixin := PcanPOrderMixin (@pickleK term_countType). *)
+(*     Canonical term_POrderType := Eval hnf in POrderType tt term_countType term_canPOrderMixin. *)
 
-      Lemma relabeling_term_preserves_is_in_ib μ trm :
-        is_in_ib  trm <-> is_in_ib (relabeling_term μ trm).
-      Proof. by case trm. Qed.
 
-      Lemma relabeling_term_preserves_is_in_i μ trm :
-        is_in_i trm <-> is_in_i (relabeling_term μ trm).
-      Proof. by case trm. Qed.
+(*   Section EqTerm. *)
+(*     Variables I B L : eqType. *)
+(*     Implicit Type trm : term I B L. *)
 
-      Lemma relabeling_term_preserves_is_in_ibl μ trm :
-        is_in_ibl trm <-> is_in_ibl (relabeling_term μ trm).
-      Proof. by case trm. Qed.
+(*     Definition eqb_term trm1 trm2 : bool := *)
+(*       match trm1, trm2 with *)
+(*       | Iri i1, Iri i2 => i1 == i2 *)
+(*       | Bnode b1, Bnode b2 => b1 == b2 *)
+(*       | Lit l1, Lit l2 => l1 == l2 *)
+(*       | _, _ => false *)
+(*       end. *)
 
-      Lemma relabeling_term_ext μ1 μ2 :
-        μ1 =1 μ2 -> forall trm, relabeling_term μ1 trm = relabeling_term μ2 trm.
-      Proof. by move=> μpweq [//| // | b] /=; rewrite μpweq. Qed.
 
-    End Relabeling_term.
-  End Poly.
+(*     Lemma term_eqP : Equality.axiom eqb_term. *)
+(*     Proof. *)
+(*       rewrite /Equality.axiom => x y. *)
+(*       apply: (iffP idP) => //= [| ->]; rewrite /eqb_term; last by case y. *)
+(*       by case: x y=> [i1|l1|b1] [i2|l2|b2] // => /eqP ->. *)
+(*     Qed. *)
 
-  Section EqTerm.
-    Variables I B L : eqType.
-    Implicit Type trm : term I B L.
 
-    Definition eqb_term trm1 trm2 : bool :=
-      match trm1, trm2 with
-      | Iri i1, Iri i2 => i1 == i2
-      | Bnode b1, Bnode b2 => b1 == b2
-      | Lit l1, Lit l2 => l1 == l2
-      | _, _ => false
-      end.
+(*     Canonical term_eqType := EqType (term I B L) (EqMixin term_eqP). *)
 
-    Lemma term_eqP : Equality.axiom eqb_term.
-    Proof.
-      rewrite /Equality.axiom => x y.
-      apply: (iffP idP) => //= [| ->]; rewrite /eqb_term; last by case y.
-      by case: x y=> [i1|l1|b1] [i2|l2|b2] // => /eqP ->.
-    Qed.
+(*   End EqTerm. *)
+(*   Section CountTerm. *)
+(*     Variable I B L: countType. *)
+(*     Implicit Type trm : term I B L. *)
 
-    Canonical term_eqType := EqType (term I B L) (EqMixin term_eqP).
+(*     Definition code_term trm := *)
+(*       match trm with *)
+(*       | Iri i => GenTree.Node 0 (GenTree.Leaf (pickle i) :: nil) *)
+(*       | Lit l => GenTree.Node 1 (GenTree.Leaf (pickle l) :: nil) *)
+(*       | Bnode name => GenTree.Node 2 (GenTree.Leaf (pickle name) :: nil) *)
+(*       end. *)
 
-  End EqTerm.
-  Section CountTerm.
-    Variable I B L: countType.
-    Implicit Type trm : term I B L.
+(*     Definition decode_term (x : GenTree.tree nat) : option (term I B L) := *)
+(*       match x with *)
+(*       | GenTree.Node 0 (GenTree.Leaf i :: nil) => omap (@Iri I B L) (unpickle i) *)
+(*       | GenTree.Node 1 (GenTree.Leaf l :: nil) =>  omap (@Lit I B L) (unpickle l) *)
+(*       | GenTree.Node 2 (GenTree.Leaf name :: nil) => omap (@Bnode I B L) (unpickle name) *)
+(*       | _ => None *)
+(*       end. *)
 
-    Definition code_term trm :=
-      match trm with
-      | Iri i => GenTree.Node 0 (GenTree.Leaf (pickle i) :: nil)
-      | Lit l => GenTree.Node 1 (GenTree.Leaf (pickle l) :: nil)
-      | Bnode name => GenTree.Node 2 (GenTree.Leaf (pickle name) :: nil)
-      end.
+(*     Lemma cancel_code_decode : pcancel code_term decode_term. *)
+(*     Proof. case => [i | l | name] /=; by rewrite pickleK. Qed. *)
 
-    Definition decode_term (x : GenTree.tree nat) : option (term I B L) :=
-      match x with
-      | GenTree.Node 0 (GenTree.Leaf i :: nil) => omap (@Iri I B L) (unpickle i)
-      | GenTree.Node 1 (GenTree.Leaf l :: nil) =>  omap (@Lit I B L) (unpickle l)
-      | GenTree.Node 2 (GenTree.Leaf name :: nil) => omap (@Bnode I B L) (unpickle name)
-      | _ => None
-      end.
+(*     Definition term_canChoiceMixin := PcanChoiceMixin cancel_code_decode. *)
+(*     Definition term_canCountMixin := PcanCountMixin cancel_code_decode. *)
 
-    Lemma cancel_code_decode : pcancel code_term decode_term.
-    Proof. case => [i | l | name] /=; by rewrite pickleK. Qed.
+(*     Canonical term_choiceType := Eval hnf in ChoiceType (term I B L) term_canChoiceMixin. *)
+(*     Canonical term_countType := Eval hnf in CountType (term I B L) term_canCountMixin. *)
 
-    Definition term_canChoiceMixin := PcanChoiceMixin cancel_code_decode.
-    Definition term_canCountMixin := PcanCountMixin cancel_code_decode.
+(*     Definition term_canPOrderMixin := PcanPOrderMixin (@pickleK term_countType) . *)
+(*     Canonical term_POrderType := Eval hnf in POrderType tt term_countType term_canPOrderMixin. *)
 
-    Canonical term_choiceType := Eval hnf in ChoiceType (term I B L) term_canChoiceMixin.
-    Canonical term_countType := Eval hnf in CountType (term I B L) term_canCountMixin.
+(*   End CountTerm. *)
+(* End Term. *)
 
-    Definition term_canPOrderMixin := PcanPOrderMixin (@pickleK term_countType).
-    Canonical term_POrderType := Eval hnf in POrderType tt term_countType term_canPOrderMixin.
-
-  End CountTerm.
-End Term.
-
-  Arguments Iri {I B L}.
-  Arguments Lit {I B L}.
-  Arguments Bnode {I B L}.
+(*   Arguments Iri {I B L}. *)
+(*   Arguments Lit {I B L}. *)
+(*   Arguments Bnode {I B L}. *)
