src/Triple.v
@@ -4,163 +4,153 @@ Unset Strict Implicit.
 Unset Printing Implicit Defensive.
 From RDF Require Import Term.
 
-Section Triple.
 
-  Record triple (I B L : Type) := mkTriple { subject : (term I B L)
-                                           ; predicate : (term I B L)
-                                           ; object: (term I B L)
-                                           ; subject_in_IB: is_in_ib subject
-                                           ; predicate_in_I: is_in_i predicate
-                                           ; object_in_IBL: is_in_ibl object
-                                   }.
+Record triple (I B L : Type) :=
+  mkTriple
+    { subject : (term I B L)
+    ; predicate : (term I B L)
+    ; object: (term I B L)
+    ; subject_in_IB: is_in_ib subject
+    ; predicate_in_I: is_in_i predicate
+ (* ; object_in_IBL: is_in_ibl object *)
+    }.
 
-  Lemma triple_inj (I B L : Type) (t1 t2 : triple I B L) :
-    subject t1 = subject t2 ->
-    predicate t1 = predicate t2 ->
-    object t1 = object t2 ->
-    t1 = t2.
-  Proof.
-    case: t1 t2 => [s1 p1 o1 sin1 pin1 oin1] [s2 p2 o2 sin2 pin2 oin2] /= seq peq oeq.
-    subst. by f_equal; apply eq_irrelevance.
-  Qed.
+Lemma triple_inj (I B L : Type) (t1 t2 : triple I B L) :
+  subject t1 = subject t2 ->
+  predicate t1 = predicate t2 ->
+  object t1 = object t2 ->
+  t1 = t2.
+Proof.
+case: t1 t2 => [s1 p1 o1 sin1 pin1] [s2 p2 o2 sin2 pin2] /= seq peq oeq.
+subst; congr mkTriple; exact: eq_irrelevance.
+Qed.
 
-  Section PolyTriple.
+Section PolyTriple.
 
-    Variables I B L : Type.
-    Implicit Type t : triple I B L.
+Variables I B L : Type.
+Implicit Type t : triple I B L.
 
-    Definition is_ground_triple t : bool:=
-      let (s,p,o,_,_,_) := t in
-      ~~ (is_bnode s || is_bnode p || is_bnode o).
+Definition is_ground_triple t : bool:=
+  let (s,p,o,_,_) := t in
+  ~~ (is_bnode s || is_bnode p || is_bnode o).
 
-    Definition relabeling_triple (B' B'': Type) (μ : B' -> B'')
-               (t : triple I B' L) : triple I B'' L :=
-      let (s,p,o,sin,pin,oin) := t in
-      mkTriple ((iffLR (relabeling_term_preserves_is_in_ib μ s)) sin)
-               ((iffLR (relabeling_term_preserves_is_in_i μ p)) pin)
-               ((iffLR (relabeling_term_preserves_is_in_ibl μ o)) oin).
+Definition relabeling_triple B1 B2 (μ : B1 -> B2) (t : triple I B1 L) : triple I B2 L :=
+  let (s, p, o, sin, pin) := t in
+  mkTriple (relabeling_term μ o)
+           ((iffLR (relabeling_term_preserves_is_in_ib μ s)) sin)
+           ((iffLR (relabeling_term_preserves_is_in_i μ p)) pin).
 
-    Lemma relabeling_triple_id t : relabeling_triple id t = t.
-    Proof.
-      case t => [s p o sin pin oin] /=. apply triple_inj => /=; by apply relabeling_term_id. Qed.
+Lemma relabeling_triple_id t : relabeling_triple id t = t.
+Proof. by case t => * /=; apply triple_inj; apply relabeling_term_id. Qed.
 
-    Lemma relabeling_triple_comp (B' B'' : Type) (μ1 : B -> B') (μ2 : B' -> B'') t :
-      relabeling_triple (μ2 \o μ1) t = relabeling_triple μ2 (relabeling_triple μ1 t).
-    Proof. by case t=> [s p o sin pin oin] ;apply triple_inj ; rewrite /= relabeling_term_comp. Qed.
+Lemma relabeling_triple_comp (B1 B2 : Type) (μ1 : B -> B1) (μ2 : B1 -> B2) t :
+  relabeling_triple (μ2 \o μ1) t = relabeling_triple μ2 (relabeling_triple μ1 t).
+Proof. by case t=> * ; apply: triple_inj ; rewrite /= relabeling_term_comp. Qed.
 
-    Section Relabeling_triple.
-      Variable B' : Type.
-      Implicit Type μ : B -> B'.
+Section Relabeling_triple.
 
-      Lemma relabeling_triple_preserves_is_in_ib μ t :
-        is_in_ib (subject t) <-> is_in_ib (subject (relabeling_triple μ t)).
-      Proof. by case t => s /= _ _ _ _ _; apply relabeling_term_preserves_is_in_ib. Qed.
+Variable B1 : Type.
+Implicit Type μ : B -> B1.
+  
+Lemma relabeling_triple_preserves_is_in_ib μ t :
+  is_in_ib (subject t) <-> is_in_ib (subject (relabeling_triple μ t)).
+Proof. by case t => s /= *; apply: relabeling_term_preserves_is_in_ib. Qed.
+  
+Lemma relabeling_triple_preserves_is_in_i μ t :
+  is_in_i (predicate t) <-> is_in_i (predicate (relabeling_triple μ t)).
+Proof. by case t => ? p /= *; apply: relabeling_term_preserves_is_in_i. Qed.
 
-      Lemma relabeling_triple_preserves_is_in_i μ t :
-        is_in_i (predicate t) <-> is_in_i (predicate (relabeling_triple μ t)).
-      Proof. by case t => _ p /= _ _ _ _; apply relabeling_term_preserves_is_in_i. Qed.
+(* Lemma relabeling_triple_preserves_is_in_ibl μ t : *)
+(*   is_in_ibl (object t) <-> is_in_ibl (object (relabeling_triple μ t)). *)
+(* Proof. by case t => ? ? o /= *; apply: relabeling_term_preserves_is_in_ibl. Qed. *)
 
-      Lemma relabeling_triple_preserves_is_in_ibl μ t :
-        is_in_ibl (object t) <-> is_in_ibl (object (relabeling_triple μ t)).
-      Proof. by case t => _ _ o /= _ _ _; apply relabeling_term_preserves_is_in_ibl. Qed.
+Lemma relabeling_triple_ext μ1 μ2:
+  μ1 =1 μ2 -> relabeling_triple μ1 =1 relabeling_triple μ2.
+Proof.
+move=> μpweq t; apply: triple_inj; case t => /= *; exact: relabeling_term_ext.
+Qed.
 
-      Lemma relabeling_triple_ext μ1 μ2:
-        μ1 =1 μ2 -> forall t, relabeling_triple μ1 t = relabeling_triple μ2 t.
-      Proof. by move=> μpweq t; apply /triple_inj; case t => /= [s p o _ _ _]; apply (relabeling_term_ext μpweq). Qed.
+End Relabeling_triple.
+End PolyTriple.
 
-    End Relabeling_triple.
-  End PolyTriple.
 
-  Section EqTriple.
-    Variable I B L : eqType.
-    Implicit Type t : triple I B L.
+Section CodeTriple.
 
-    Definition eqb_triple  t1 t2 : bool :=
-      ((subject t1) == (subject t2)) &&
-        ((predicate t1) == (predicate t2)) &&
-        ((object t1) == (object t2)).
+Variables (I B L : Type).
 
-    Lemma triple_eqP : Equality.axiom eqb_triple.
-    Proof.
-      rewrite /Equality.axiom /eqb_triple => x y.
-      apply: (iffP idP) => //= [| ->];
-                          case: x y=> [s1 p1 o1 sin1 pin1 oin1] [s2 p2 o2 sin2 pin2 oin2] //=.
-      case/andP; case/andP=> /eqP eq_s/eqP eq_p/eqP eq_o.
-      by apply triple_inj => /=.
-      by rewrite !eq_refl //.
-    Qed.
+Implicit Type tr : triple I B L.
 
-    Canonical triple_eqType := EqType (triple I B L) (EqMixin triple_eqP).
+Definition code_triple tr : (term I B L * term I B L * term I B L)%type :=
+  let: mkTriple s p o  _ _ := tr in (s, p, o).
 
-    Definition terms_triple t : seq (term I B L) :=
-      let (s,p,o,_,_,_) := t in
-      undup [:: s ; p ; o].
+Definition decode_triple (t : (term I B L * term I B L * term I B L)%type) :=
+  let: (s, p, o) := t in
+  if insub s : {? x | is_in_ib x} is Some ss then
+    if insub p : {? x | is_in_i x} is Some pp then
+      Some (mkTriple o (valP ss) (valP pp))
+    else None
+  else None.
 
-    Canonical triple_predType := PredType (pred_of_seq \o terms_triple).
+Lemma pcancel_code_decode : pcancel code_triple decode_triple.
+Proof.
+case=> s p o ibs ip /=.
+case: insubP=> [u uP us |]; last by rewrite ibs. 
+case: insubP=> [v vP vs |]; last by rewrite ip. 
+by congr Some; apply: triple_inj. 
+Qed.
 
-    (* Definition bnodes_triple t :[seq x <- terms_triple t | x is_bnode] := *)
+End CodeTriple.
+
+Definition triple_canEqMixin (I B L : eqType) := PcanEqMixin (@pcancel_code_decode I B L).
+Canonical triple_eqType (I B L : eqType) :=
+  Eval hnf in EqType (triple I B L) (triple_canEqMixin I B L).
+
+Definition triple_canChoiceMixin (I B L : choiceType) :=
+  PcanChoiceMixin (@pcancel_code_decode I B L).
+
+Canonical triple_choiceType (I B L : choiceType) :=
+  Eval hnf in ChoiceType (triple I B L) (triple_canChoiceMixin I B L).
+
+Definition triple_canCountMixin (I B L : countType) :=
+  PcanCountMixin (@pcancel_code_decode I B L).
+Canonical triple_countType (I B L : countType) :=
+  Eval hnf in CountType (triple I B L) (triple_canCountMixin I B L).
+
+Definition triple_canPOrderMixin (I B L : countType) :=
+  PcanPOrderMixin (@pickleK (triple_countType I B L)).
+
+Canonical triple_POrderType (I B L : countType) :=
+  Eval hnf in POrderType tt (triple_countType I B L) (triple_canPOrderMixin I B L).
+
+
+(* assia : below not cleaned up *)
+Section OperationsOnTriples.
+
+Variables I B L : eqType.
+Implicit Type t : triple I B L.
+
+Definition terms_triple t : seq (term I B L) :=
+  let (s,p,o,_,_) := t in undup [:: s ; p ; o].
+
+Canonical triple_predType := PredType (pred_of_seq \o terms_triple).
+
+(* Definition bnodes_triple t :[seq x <- terms_triple t | x is_bnode] := *)
     (*   undup (filter (@is_bnode _ _ _) (terms_triple t)). *)
 
-    Definition bnodes_triple t : seq (term I B L) :=
-      undup (filter (@is_bnode _ _ _) (terms_triple t)).
+Definition bnodes_triple t : seq (term I B L) :=
+  undup (filter (@is_bnode _ _ _) (terms_triple t)).
 
     
-    Definition all_bnodes_triple_is_bnode t : all (@is_bnode I B L) (bnodes_triple t).
-    Proof. rewrite /bnodes_triple -filter_undup; apply filter_all. Qed.
+Definition all_bnodes_triple_is_bnode t : all (@is_bnode I B L) (bnodes_triple t).
+Proof. rewrite /bnodes_triple -filter_undup; apply filter_all. Qed.
 
-    Definition get_b_triple t : seq B.
-    Proof. apply bnodes_triple in t as bns. 
-           elim bns => [|b bs ibs].
-           + exact [::].
-           + case b=> x. exact [::]. exact [::]. exact (undup (x::ibs)).
-    Defined.
+Definition get_b_triple t : seq B.
+Proof. apply bnodes_triple in t as bns. 
+       
+       elim bns => [|b bs ibs].
+       + exact [::].
+       + case b=> x. exact [::]. exact [::]. exact (undup (x::ibs)).
+Defined.
 
-  End EqTriple.
 
-  Section CountTriple.
-    Variables I B L : countType.
-    Implicit Type t : triple I B L.
-
-    Definition code_triple t :=
-      let (s,p,o,_,_,_) := t in
-      GenTree.Node 0 [:: (code_term s); (code_term p) ; (code_term o)].
-
-    Definition decode_triple (x : GenTree.tree nat) : option (triple I B L).
-    Proof. destruct x eqn:E.
-           - exact None.
-           - destruct n as [| n'].
-             + destruct l as [| s [| p [| o]]] eqn:size.
-               * exact None.
-               * exact None.
-               * exact None.
-               * destruct l0.
-                 -- destruct (decode_term I B L s) as [dst | ] eqn:ds;
-                      destruct (decode_term I B L p) as [dpt | ] eqn:dp;
-                      destruct (decode_term I B L o) as [ dot| ] eqn:do.
-                                                                       destruct (is_in_ib dst) eqn:iib;
-                                                                         destruct (is_in_i dpt) eqn:ii;
-                                                                         destruct (is_in_ibl dot) eqn: ibl.
-
-                                                                       ++ exact (Some (mkTriple iib ii ibl)).
-                                                                       + all: exact None.
-    Defined.
-
-    Lemma cancel_triple_encode : pcancel code_triple decode_triple.
-    Proof. case => s p o sib ii oibl. rewrite /code_triple /decode_triple.
-           have cant: forall (trm : term I B L), decode_term I B L (code_term trm) = Some trm. apply cancel_code_decode.
-           rewrite /= !cant; destruct s; destruct p ; destruct o => //=.
-           all: by f_equal; apply triple_inj.
-    Qed.
-
-    Definition triple_canChoiceMixin := PcanChoiceMixin cancel_triple_encode.
-    Definition triple_canCountMixin := PcanCountMixin cancel_triple_encode.
-
-    Canonical triple_choiceType := Eval hnf in ChoiceType (triple I B L) triple_canChoiceMixin.
-    Canonical triple_countType := Eval hnf in CountType (triple I B L) triple_canCountMixin.
-
-    Definition triple_canPOrderMixin := PcanPOrderMixin (@pickleK triple_countType).
-    Canonical triple_POrderType := Eval hnf in POrderType tt (triple I B L) triple_canPOrderMixin.
-
-  End CountTriple.
-End Triple.
-
+End OperationsOnTriples.
